thys/core_pre.thy
@@ -23,25 +23,30 @@ translations
 
 subsubsection {* Generalized While Combinator *}
 
+text {* In the Rust intermediate representation, every loop is represented by the unconditional
+  @{verbatim loop} control structure. We accordingly generalize Isabelle's While combinator. *}
+
 datatype loop_control = Continue | Break
 
 definition loop :: "('state \<Rightarrow> 'state \<times> loop_control) \<Rightarrow> 'state \<Rightarrow> 'state option" where
   "loop l s \<equiv> map_option (\<lambda>(s,s',c). s')
     (while_option (\<lambda>(s,s',c). c = Continue) (\<lambda>(s,s',c). (s',(l s'))) (s,(l s)))"
 
+text {* Extend @{term loop} to partial loop body functions. *}
+
 definition loop' :: "('state \<Rightarrow> ('state \<times> loop_control) option) \<Rightarrow> 'state \<Rightarrow> 'state option" where
   "loop' l s = Option.bind (
-    loop (\<lambda>s. case s of
-      None \<Rightarrow> (None, Break)
-    | Some s \<Rightarrow> (case l s of
-        None \<Rightarrow> (Some s, Break)
-      | Some (s',c) \<Rightarrow> (Some s',c)))
+    loop (\<lambda>s. case l (the s) of
+        None \<Rightarrow> (Some (the s), Break)
+      | Some (s',c) \<Rightarrow> (Some s',c))
     (Some s)
   ) id"
 
 subsection {* Types *}
 
 subsubsection {* Machine Types *}
+
+text {* Isabelle's Word library provides some nice support for fixed-size integers. *}
 
 type_synonym u8 = "8 word"
 type_synonym u16 = "16 word"
@@ -53,29 +58,34 @@ abbreviation "u16 n \<equiv> word_of_int n::u16"
 abbreviation "u32 n \<equiv> word_of_int n::u32"
 abbreviation "u64 n \<equiv> word_of_int n::u64"
 
-lift_definition uint_with_overflow :: "(int \<Rightarrow> int \<Rightarrow> int) \<Rightarrow> 'a::len0 word \<Rightarrow> 'a word \<Rightarrow> 'a word \<times> bool" is "\<lambda>f n m.
-  let i = f (uint n) (uint m)in
+lift_definition unsigned_with_overflow :: "(int \<Rightarrow> int \<Rightarrow> int) \<Rightarrow> 'a::len0 word \<Rightarrow> 'a word \<Rightarrow> 'a word \<times> bool" is "\<lambda>f n m.
+  let i = f (uint n) (uint m) in
   (i, uint (word_of_int i::'a word) \<noteq> i)" .
 
-lift_definition uint_checked :: "(int \<Rightarrow> int \<Rightarrow> int) \<Rightarrow> 'a::len0 word \<Rightarrow> 'a word \<Rightarrow> 'a word option" is "\<lambda>f n m. case uint_with_overflow f n m of
+text {* In Rust, overflowing arithmetic operations are undefined behavior, which we model as returning @{term None}. *}
+
+lift_definition unsigned_checked :: "(int \<Rightarrow> int \<Rightarrow> int) \<Rightarrow> 'a::len0 word \<Rightarrow> 'a word \<Rightarrow> 'a word option" is "\<lambda>f n m. case unsigned_with_overflow f n m of
   (n, False) \<Rightarrow> Some n
 | (_, True)  \<Rightarrow> None" .
 
-abbreviation "checked_add \<equiv> uint_checked (op +)"
-abbreviation "checked_sub \<equiv> uint_checked (op -)"
-abbreviation "checked_mul \<equiv> uint_checked (op *)"
-abbreviation "checked_div \<equiv> uint_checked (op div)"
-abbreviation "checked_mod \<equiv> uint_checked (op mod)"
+abbreviation "checked_add \<equiv> unsigned_checked (op +)"
+abbreviation "checked_sub \<equiv> unsigned_checked (op -)"
+abbreviation "checked_mul \<equiv> unsigned_checked (op *)"
+abbreviation "checked_div \<equiv> unsigned_checked (op div)"
+abbreviation "checked_mod \<equiv> unsigned_checked (op mod)"
 
-(* TODO *)
-definition "checked_shl (a::'a::len word) b = Some (a << (unat b))"
-definition "checked_shr (a::'a::len word) b = Some (a >> (unat b))"
+(* TODO
+definition "unsigned_checked_shl (a::'a::len word) b = Some (a << (unat b))"
+definition "unsigned_checked_shr (a::'a::len word) b = Some (a >> (unat b))"
+*)
 
 subsubsection {* Machine-Dependent Integer Types *}
 
+text {* We model the target system's native byte size as an axiomatic constant with a reasonable
+  lower bound (met by all target architectures currently supported by @{verbatim rustc}). *}
+
 consts native_bs :: nat
 
-(* let's be somewhat realistic *)
 specification (native_bs) native_bs_min: "native_bs \<ge> 32"
 by auto
 
@@ -94,21 +104,32 @@ type_synonym usize = "native_bs word"
 
 abbreviation "usize n \<equiv> word_of_int n::usize"
 
+(*
 subsubsection {* Manually-Translated Types *}
 
 typedef 'a slice = "{xs::'a list. length xs < 2^native_bs}"
 by (rule exI[where x="[]"], simp)
+*)
 
 subsection {* Functions *}
 
 subsubsection {* Intrinsics *}
 
-abbreviation "core_intrinsics_add_with_overflow n m \<equiv> Some (uint_with_overflow (op +) n m)"
-abbreviation "core_intrinsics_sub_with_overflow n m \<equiv> Some (uint_with_overflow (op -) n m)"
-abbreviation "core_intrinsics_mul_with_overflow n m \<equiv> Some (uint_with_overflow (op *) n m)"
+abbreviation "core_intrinsics_add_with_overflow n m \<equiv> Some (unsigned_with_overflow (op +) n m)"
+abbreviation "core_intrinsics_sub_with_overflow n m \<equiv> Some (unsigned_with_overflow (op -) n m)"
+abbreviation "core_intrinsics_mul_with_overflow n m \<equiv> Some (unsigned_with_overflow (op *) n m)"
 
 subsubsection {* Manually-Translated Functions *}
 
-definition[simp]: "core_mem_swap x y = Some ((),y,x)"
+text {* The original implementation of @{verbatim "core::mem::swap"} uses (via unsafe code) the @{verbatim uninitialized}
+  intrinsic. Since it is not clear whether or how we want to support uninitialized memory, we instead
+  give a straight-forward manual implementation. *}
+
+definition [simp]: "core_mem_swap x y = Some ((),y,x)"
 
 end
+
+section {* Transpilation of the \emph{core} crate *}
+
+text {* This section merely contains the (transitive) dependencies of the single for loop we want to verify. Still, you might want
+  to skip to the \hyperref[sec:core]{next section}. *}
