thys/core.thy
@@ -1,17 +1,23 @@
+section \<open> Proofs about the \emph{core} crate \<close>
+
+text_raw \<open> \label{sec:core} \<close>
+
 theory core
 imports
   core_export
 begin
 
+subsection \<open> Lemmas that should be in HOL/Library \<close>
+
 definition "all_option P = case_option False P"
 
-lemma all_option_Some[simp]: "all_option P (Some x) = P x"
+lemma all_option_Some [simp]: "all_option P (Some x) = P x"
 by (simp add: all_option_def)
 
-lemma all_option_None[simp]: "\<not>all_option P None"
+lemma all_option_None [simp]: "\<not>all_option P None"
 by (simp add: all_option_def)
 
-lemma all_optionE[elim!]:
+lemma all_optionE [elim!]:
   assumes "all_option P x"
   obtains x' where "x = Some x'" "P x'"
 using assms by (cases x; simp)
@@ -21,7 +27,7 @@ by (cases x; simp)
 
 lemma all_option_eq: "all_option (\<lambda>x. x = y) x \<longleftrightarrow> x = Some y"
 by (cases x; simp)
-
+ 
 theorem while_opt_rule_lemma:
   assumes invariant: "!!s. P s ==> b s ==> P (c s)"
     and terminate: "!!s. P s ==> \<not> b s ==> Q s"
@@ -49,10 +55,15 @@ theorem while_opt_rule:
   apply blast
   done
 
+subsection \<open> Lemmas about @{term loop} \<close>
+
+lemma not_loop_control [simp]: "l \<noteq> Continue \<Longrightarrow> l = Break" "l \<noteq> Break \<Longrightarrow> l = Continue"
+  by (cases l, simp_all)+
+
 lemma loop_rule:
   assumes "P s"
-  assumes "\<And>s s'. P s \<Longrightarrow> l s = (s',True) \<Longrightarrow> P s'" "\<And>s s'. P s \<Longrightarrow> l s = (s',False) \<Longrightarrow> Q s'"
-  assumes "wf r" "\<And>s s'. P s \<Longrightarrow> l s = (s',True) \<Longrightarrow> (s', s) \<in> r"
+  assumes "\<And>s s'. P s \<Longrightarrow> l s = (s',Continue) \<Longrightarrow> P s'" "\<And>s s'. P s \<Longrightarrow> l s = (s',Break) \<Longrightarrow> Q s'"
+  assumes "wf r" "\<And>s s'. P s \<Longrightarrow> l s = (s',Continue) \<Longrightarrow> (s', s) \<in> r"
   shows "all_option Q (loop l s)"
 proof-
   let ?r' = "{((s\<^sub>1, l s\<^sub>1), (s\<^sub>2, l s\<^sub>2)) | s\<^sub>1 s\<^sub>2. (s\<^sub>1,s\<^sub>2) \<in> r}"
@@ -67,8 +78,8 @@ qed
 
 lemma loop'_rule:
   assumes "P s"
-  assumes "\<And>s. P s \<Longrightarrow> l s \<noteq> None" "\<And>s s'. P s \<Longrightarrow> l s = Some (s',True) \<Longrightarrow> P s'" "\<And>s s'. P s \<Longrightarrow> l s = Some (s',False) \<Longrightarrow> Q s'"
-  assumes "wf r" "\<And>s s'. P s \<Longrightarrow> l s = Some (s',True) \<Longrightarrow> (s', s) \<in> r"
+  assumes "\<And>s. P s \<Longrightarrow> l s \<noteq> None" "\<And>s s'. P s \<Longrightarrow> l s = Some (s',Continue) \<Longrightarrow> P s'" "\<And>s s'. P s \<Longrightarrow> l s = Some (s',Break) \<Longrightarrow> Q s'"
+  assumes "wf r" "\<And>s s'. P s \<Longrightarrow> l s = Some (s',Continue) \<Longrightarrow> (s', s) \<in> r"
   shows "all_option Q (loop' l s)"
 proof-
   let ?r' = "{(Some s\<^sub>1, Some s\<^sub>2) | s\<^sub>1 s\<^sub>2. (s\<^sub>1,s\<^sub>2) \<in> r}"
@@ -83,32 +94,39 @@ qed
 declare Let_def[simp] Option.bind_eq_None_conv[simp] semiring_numeral_class.power_numeral[simp del]
 declare not_None_eq[iff del]
 
-lemma checked_add[simp]: "checked_add (n::'bs::len word) m = (if n \<le> n + m then Some (n+m) else None)"
-apply (auto simp add: uint_checked_def uint_with_overflow_def uint_word_of_int int_mod_lem[symmetric] split: bool.splits)
-  apply uint_arith
- apply uint_arith
- apply (auto simp add: uint_word_of_int int_mod_lem[symmetric])[1]
-apply uint_arith
-done
-
-lemma checked_mul: "checked_mul (n::'bs::len word) m = (if uint n * uint m < 2^len_of TYPE('bs) then Some (n*m) else None)"
-  by (auto simp add: uint_checked_def uint_with_overflow_def uint_word_of_int int_mod_lem[symmetric] word_mult_def split: bool.splits)
+subsection \<open> Arithmetic operations \<close>
 
 context
   fixes a b c :: "'a::len word"
 begin
-  lemma word_succ_no_overflow[simp]: "a < b \<Longrightarrow> a \<le> a + 1" by uint_arith
+  lemma checked_add [simp]: "checked_add a b = (if a \<le> a + b then Some (a+b) else None)"
+  apply (auto simp add: unsigned_checked_def unsigned_with_overflow_def uint_word_of_int int_mod_lem[symmetric] split: bool.splits)
+    apply uint_arith
+   apply uint_arith
+   apply (auto simp add: uint_word_of_int int_mod_lem[symmetric])[1]
+  apply uint_arith
+  done
+  
+  lemma checked_mul: "checked_mul a b = (if uint a * uint b < 2^len_of TYPE('a) then Some (a*b) else None)"
+    by (auto simp add: unsigned_checked_def unsigned_with_overflow_def uint_word_of_int int_mod_lem[symmetric] word_mult_def split: bool.splits)
+
+  lemma word_succ_no_overflow [simp]: "a < b \<Longrightarrow> a \<le> a + 1" by uint_arith
 
   lemma word_le_succ_trans: "a < b \<Longrightarrow> c \<le> a \<Longrightarrow> c \<le> a + 1" by uint_arith
 end
 
+subsection \<open> Loops over @{verbatim u32} ranges \<close>
+
+text \<open> Because the following lemmas reference specific trait implementations for @{verbatim u32}, it is not
+  clear how they could be generalized to other numeric types. \<close>
+
 lemma loop_range_u32:
   assumes "P l res\<^sub>0"
-  assumes "\<And>i res iter. \<lbrakk>l \<le> i; i < r; P i res\<rbrakk> \<Longrightarrow> f i res iter = Some ((g i res, iter), True)"
+  assumes "\<And>i res iter. \<lbrakk>l \<le> i; i < r; P i res\<rbrakk> \<Longrightarrow> f i res iter = Some ((g i res, iter), Continue)"
   assumes "\<And>i res iter. \<lbrakk>l \<le> i; i < r; P i res\<rbrakk> \<Longrightarrow> P (i + 1) (g i res)"
   shows "all_option (P (max l r) \<circ> fst) (loop' (\<lambda>(res, iter).
                   do (t6, iter) \<leftarrow> (core_iter_ops_Range_A__Iterator_next (core_num_u32_One) (core_iter_u32_Step) (core_ops___b_u32_Add___a_u32) iter);
-                  case t6 of core_option_Option_None \<Rightarrow> Some ((res, iter), False)
+                  case t6 of core_option_Option_None \<Rightarrow> Some ((res, iter), Break)
                      | core_option_Option_Some i \<Rightarrow> f i res iter)
          (res\<^sub>0, core_ops_Range.make l r))"
 apply (rule loop'_rule[where P="\<lambda>s. case s of (res, iter) \<Rightarrow>
@@ -124,15 +142,55 @@ apply (clarsimp simp: assms(2) split: split_if_asm intro!: unat_mono)
 apply uint_arith
 done
 
+text \<open> A variant of @{text loop_range_u32} that is easier to unify with a goal \<close>
+
 lemma loop_range_u32':
   assumes "body = (\<lambda>(res, iter).
                   do (t6, iter) \<leftarrow> core_iter_ops_Range_A__Iterator_next core_num_u32_One core_iter_u32_Step core_ops___b_u32_Add___a_u32 iter;
-                  case t6 of core_option_Option_None \<Rightarrow> Some ((res, iter), False)
+                  case t6 of core_option_Option_None \<Rightarrow> Some ((res, iter), Break)
                      | core_option_Option_Some i \<Rightarrow> f i res iter)"
-  assumes "\<And>i res iter. \<lbrakk>l \<le> i; i < r; P i res\<rbrakk> \<Longrightarrow> f i res iter = Some ((g i res, iter), True) \<and> P (i + 1) (g i res)"
+  assumes "\<And>i res iter. \<lbrakk>l \<le> i; i < r; P i res\<rbrakk> \<Longrightarrow> f i res iter = Some ((g i res, iter), Continue) \<and> P (i + 1) (g i res)"
   assumes "\<And>x. P (max l r) (fst x) \<Longrightarrow> P' (Some x)"
   assumes "P l res\<^sub>0"
   shows "P' (loop' body (res\<^sub>0, core_ops_Range.make l r))"
 by (cut_tac loop_range_u32[of P l res\<^sub>0 r f g]) (auto simp: assms[unfolded assms(2)])
 
 end
+
+section \<open> Transpilation of the \emph{examples} crate \<close>
+
+text \<open> Original code:
+
+  \begin{lstlisting}
+fn fac(n: u32) -> u32 {
+    let mut res = 1;
+    for i in 2..n+1 {
+        res *= i;
+    }
+    res
+}
+  \end{lstlisting}
+
+  Expanded code:
+
+  \begin{lstlisting}
+fn fac(n: u32) -> u32 {
+    let mut res = 1;
+    {
+        let _result =
+            match ::core::iter::IntoIterator::into_iter(2..n + 1) {
+                mut iter =>
+                loop  {
+                    match ::core::iter::Iterator::next(&mut iter) {
+                        ::core::option::Option::Some(i) => { res *= i; }
+                        ::core::option::Option::None => break ,
+                    }
+                },
+            };
+        _result
+    }
+    res
+}
+  \end{lstlisting}
+
+\<close>
