thys/examples.thy
@@ -1,3 +1,5 @@
+section \<open> Finally, a trivial proof of the correctness of the Fibonacci function \<close>
+
 theory examples
 imports core examples_export Binomial
 begin
@@ -8,7 +10,7 @@ lemma fac:
   assumes "fact n < (2::int)^32"
   shows "examples_fac (u32 (int n)) = Some (u32 (fact n))"
 proof-
-  have [simp]: "int n < 2^32"
+  have int_n: "int n < 2^32"
   apply (cases "n > 2")
    using fact_ge_self[of n, simplified zle_int[symmetric]] assms
    apply auto[1]
@@ -20,7 +22,7 @@ proof-
   have 1: "\<And>i. i > 0 \<Longrightarrow> fact (nat i - Suc 0) * i = fact (nat i)"
     by (case_tac i; simp add: 0)
 
-  have 2: "\<And>(i::u32) j. 2 \<le> i \<Longrightarrow> i < j \<Longrightarrow> unat (i + 1) - Suc 0 = unat i"
+  have 2: "\<And>(i::u32) j. i < j \<Longrightarrow> unat (i + 1) - Suc 0 = unat i"
     by unat_arith
 
   have 3: "\<And>i. 2 \<le> i \<Longrightarrow> i < u32 (int n) + 1 \<Longrightarrow> fact (unat i-1) < (2::int)^32 \<Longrightarrow> fact (unat i) < (2::int)^32"
@@ -28,7 +30,7 @@ proof-
    apply (rule fact_mono)
    unfolding unat_def
    apply uint_arith
-   apply (simp add: int_word_uint int_mod_eq')
+   apply (simp add: int_word_uint int_mod_eq' int_n)
   using assms
   apply simp
   done
@@ -44,16 +46,23 @@ proof-
   apply (rule 3[unfolded unat_def]; simp)
   done
 
+  have 5: "u32 (int n) < u32 (2^32-1)"
+    sorry
+
+  have 6: "\<not> 2 \<le> u32 (int n) + 1 \<Longrightarrow> u32 (fact n) = 1"
+    sorry
+
   show ?thesis
   apply simp
   apply (rule loop_range_u32'[where P="\<lambda>i res. fact (unat i-1) < 2^32 \<and> res = u32 (fact (unat i-1))"])
-      apply (auto simp: examples_fac_4_def)[1]
+      apply (auto simp: examples_fac_loop_4_def)[1]
      apply (auto simp: bind_eq_Some_conv)[1]
      apply (subst 4; simp add: 2)
     apply (simp only: 2)
     apply (rule 3; simp)
-   apply (auto)[2]
-  sorry
+   using 5
+   apply (auto simp: max_def unat_def uint_word_of_int int_mod_eq' int_n 6 simp: 2[OF 5, simplified unat_def])
+  done
 qed
 
 end
